
# 97. Interleaving String

  

## Question


Given strings  `s1`,  `s2`, and  `s3`, find whether  `s3`  is formed by an  **interleaving**  of  `s1`  and  `s2`.

An  **interleaving**  of two strings  `s`  and  `t`  is a configuration where they are divided into  **non-empty**  substrings such that:

-   `s = s1  + s2  + ... + sn`
-   `t = t1  + t2  + ... + tm`
-   `|n - m| <= 1`
-   The  **interleaving**  is  `s1  + t1  + s2  + t2  + s3  + t3  + ...`  or  `t1  + s1  + t2  + s2  + t3  + s3  + ...`

**Note:**  `a + b`  is the concatenation of strings  `a`  and  `b`.

**Example 1:**

![](https://assets.leetcode.com/uploads/2020/09/02/interleave.jpg)

**Input:** s1 = "aabcc", s2 = "dbbca", s3 = "aadbbcbcac"
**Output:** true

**Example 2:**

**Input:** s1 = "aabcc", s2 = "dbbca", s3 = "aadbbbaccc"
**Output:** false

**Example 3:**

**Input:** s1 = "", s2 = "", s3 = ""
**Output:** true

**Constraints:**

-   `0 <= s1.length, s2.length <= 100`
-   `0 <= s3.length <= 200`
-   `s1`,  `s2`, and  `s3`  consist of lowercase English letters.

**Follow up:**  Could you solve it using only  `O(s2.length)`  additional memory space?
## Solution

  

### Approach 1: DP

#### Intuition
For each char in s3, we need to choose either current char in s1 or s2 and move our pointer.

The hard part is when we have duplicate chars from s1 and s2, and we can't really make a decision. For that part, we can't avoid going back if we made a mistake. But we can use memorization to avoid duplicated calculations. 

We can use recursion to help make the logic clearer.

#### Algorithm
1. Dp function returns whether it returns true for `(i, j)`, for `S3[:(i+j)]` is formed by an  **interleaving**  of `s1[:i], s2[:j]`
2. Check whether we should even proceed with dp (based on length)
3. Start calling dp with `(len(s1) - 1, len(s2) - 1)`

#### Code
```python
class Solution:
    def isInterleave(self, s1: str, s2: str, s3: str) -> bool:
        @lru_cache(None)
        def dp(i, j):
            if i == -1 and j == -1: return True
            return (j >= 0 and s2[j] == s3[i+j+1] and dp(i, j-1)) or (i >= 0 and s1[i] == s3[i+j+1] and dp(i-1,j))
        return len(s1) + len(s2) == len(s3) and dp(len(s1) - 1, len(s2) - 1)
```

#### Complexity Analysis

  

-  **Time Complexity:** O(mn), all combinations are calculated once
  

-  **Space Complexity:** O(mn), our memorized recursion calls